README.md
@@ -1,39 +1,10 @@
-# CompCert
-The formally-verified C compiler.
+# Nominal CompCert
 
 ## Overview
-The CompCert C verified compiler is a compiler for a large subset of the
-C programming language that generates code for the PowerPC, ARM, x86 and
-RISC-V processors.
+We replaced the "nextblock" design in CompCert by "support and freshness" which comes from Nominal Technique.
 
-The distinguishing feature of CompCert is that it has been formally
-verified using the Coq proof assistant: the generated assembly code is
-formally guaranteed to behave as prescribed by the semantics of the
-source C code.
+This version uses Module Type to describe the necessary properties (definitions and theorems) of "block" and "sup" Type for the original compilation pass. 
 
-For more information on CompCert (supported platforms, supported C
-features, installation instructions, using the compiler, etc), please
-refer to the [Web site](https://compcert.org/) and especially
-the [user's manual](https://compcert.org/man/).
+We have repaired the whole proof using "Declare Module sup:SUP (block:BLOCK)". We have also made the compiler available using "positive" and "positive list" to realize "block" and "sup". While the code is the same except the definition of these two Modules. 
 
-## License
-CompCert is not free software.  This non-commercial release can only
-be used for evaluation, research, educational and personal purposes.
-A commercial version of CompCert, without this restriction and with
-professional support and extra features, can be purchased from
-[AbsInt](https://www.absint.com).  See the file `LICENSE` for more
-information.
-
-## Copyright
-The CompCert verified compiler is Copyright Institut National de
-Recherche en Informatique et en Automatique (INRIA) and 
-AbsInt Angewandte Informatik GmbH.
-
-
-## Contact
-General discussions on CompCert take place on the
-[compcert-users@inria.fr](https://sympa.inria.fr/sympa/info/compcert-users)
-mailing list.
-
-For inquiries on the commercial version of CompCert, please contact
-info@absint.com
+We optimistically believe that we can design different "block" and "sup" types which satisfy our signature to carry more information and improve/extend the original CompCert without breaking the proves we do not concern.
